more thing

Picinae_calling.v
@@ -1116,7 +1116,7 @@ Definition trace_program_step_at (vars: list var) (p: program)
           | Some (sz, q) =>
               (* Sanity check for if we have already visited this address *)
               match ts addr with
-              | None => None
+              | None => Some (ts, changed)
               | Some δ_a =>
                   match simple_trace_stmt δ_a q with
                   | None => None
@@ -1233,7 +1233,7 @@ Proof.
     destruct (a1 == a1'); try discriminate. subst. assumption.
 Admitted.
 
-Definition hintDelta (hints: program → addr → trace_states → option (trace_states * bool))  (p : program) : 
+Definition hintDelta (hints: (store → addr → option (N * stmt)) → addr → (addr → option store_delta) -> option ((addr → option store_delta) * bool))  (p : store → addr → option (N * stmt)) : 
     Prop := forall a_new ts b,
    hints p a_new ts = Some (ts, b) -> (forall a, exists δ1, ts a = Some δ1).
  
@@ -1278,20 +1278,39 @@ Proof.
       destruct join_states_if_changed eqn:H_jsic in H; inversion H.
         subst. apply IHl in H_fr. inversion H_fr. reflexivity.
       inversion H. subst. apply IHl in H_fr. inversion H_fr. reflexivity.
-Qed.  
-(*
-Theorem trace_program_step_at_nochange: forall reachable_addrs p hints ts vars t,
-fold_right (trace_program_step_at vars p hints) (Some (ts, false)) reachable_addrs = Some (t, false) -> t = ts.
+Qed. 
+Theorem trace_program_step_at_nochange: forall reachable_addrs vars p hints t ts, 
+  fold_right (trace_program_step_at vars p hints) (Some (t, false)) reachable_addrs = Some (ts, false) -> t = ts.
 Proof.
-  induction reachable_addrs.
+  induction reachable_addrs.  
     intros. simpl in H. inversion H. reflexivity.
-
-    intros. simpl in H. destruct fold_right eqn:H_fr in H.
-    unfold trace_program_step_at in H. 
-      destruct p0. destruct hints. 
-        destruct p0. in H.
+    intros. simpl in H. destruct fold_right eqn:H_fr; try solve [inversion H].  
+      unfold trace_program_step_at in H.
+      destruct p0 eqn:H_p0. unfold trace_program_step_at in H.
+      destruct hints eqn:H_hint in H.
+        admit.
+    destruct p eqn:H_p; try solve [inversion H]. destruct p1; try solve [inversion H]. 
+    destruct t0 eqn:H_t. 
+      destruct simple_trace_stmt eqn:H_sts; try discriminate. inversion H. apply process_state_vars_nochange in H1. 
+         inversion H1. subst. eapply IHreachable_addrs. apply H_fr. 
+      inversion H. subst. eapply IHreachable_addrs.  apply H_fr.
+Admitted.
+(*MARKK*)
+Theorem test2: forall (p : store → addr → option (N * stmt)) hints reachable ts p vars q sz s2 a2
+    (TPO : expand_trace_program vars p hints reachable ts = Some (ts, false))
+    (HINT: hintDelta hints p)
+    (LU : sub_prog p (set_elems reachable) s2 a2 = Some (sz, q)),
+    exists δ, ts a2 = Some δ.
+Proof.
+ intros. revert TPO LU. revert ts vars q sz s2 a2. destruct reachable as [reachable_addrs UNIQ_reachable_addrs]. 
+  (*intros.  unfold expand_trace_program in TPO. unfold trace_program_step_at in TPO.*)
+  induction reachable_addrs.
+  - intros. subst. simpl in TPO. unfold sub_prog in LU. simpl in LU. inversion LU.
+  - intros. 
+    unfold expand_trace_program in *.  simpl in *. destruct fold_right eqn:H_fr; try solve [inversion TPO].  
+    destruct p1. 
+ 
 Qed.
- *)
 (*MARKK*)
 Theorem test: forall (p : store → addr → option (N * stmt)) hints reachable ts p vars q sz s2 a2
     (TPO : expand_trace_program vars p hints reachable ts = Some (ts, false))
@@ -1308,8 +1327,8 @@ Proof.
     unfold expand_trace_program in *. simpl in *. 
     destruct fold_right eqn:H_fr; try solve [inversion TPO].  
     destruct p1 eqn:H_p1. unfold trace_program_step_at in TPO.
-    destruct hints eqn:H_hint in TPO. admit.
-    (*unfold hintDelta in HINT. destruct p2. inversion TPO. subst. eapply HINT in H_hint. (*hints will have to be asserted*). simpl in TPO. *)
+    destruct hints eqn:H_hint in TPO. 
+    unfold hintDelta in HINT. destruct p2. eapply HINT. apply H_hint. (*hints will have to be asserted*). simpl in TPO.
     destruct p0 eqn:H_p; try solve [inversion TPO]. destruct p1; try solve [inversion TPO]. 
     destruct p2 eqn:H_p2. subst.  destruct t eqn:H_t; try solve [inversion TPO]. 
     destruct simple_trace_stmt eqn:H_sts; try solve [inversion TPO]. inversion TPO.
@@ -1319,7 +1338,7 @@ Proof.
     apply iseqb_iff_eq in H. subst. split with (x:= s0). apply H_t. 
     eapply IHreachable_addrs.
       inversion UNIQ_reachable_addrs. subst. apply H3. apply H_fr. unfold sub_prog. rewrite -> H. apply LU.
-Admitted.
+Qed.
 
 Theorem expand_trace_program_steady_correct_n: forall p vars hints reachable ts
   h a0 s0 
